theories/decidability.v
@@ -1,0 +1,378 @@
+From stdpp Require Import relations finite fin.
+From Coq Require Import ssreflect.
+From Coq Require Import Recdef.
+From Coq.Program Require Import Wf.
+From ambig Require Import util grammar acyclic.
+
+Section decidability.
+
+  Variable Σ N : Type.
+  Context `{EqDecision Σ}.
+  Context `{EqDecision N}.
+
+  Global Instance token_eq_dec : EqDecision (token Σ).
+  Proof.
+    intros [a1 p1] [a2 p2].
+    destruct (decide (a1 = a2 ∧ p1 = p2)); [left | right]; naive_solver.
+  Qed.
+
+  Variable G : grammar Σ N.
+  Context `{acyclic G}.
+
+  (* Implicit Type A Al Ar B Bl Br : N. *)
+  Implicit Type w h : sentence Σ.
+
+  Definition sig_lt : relation (sentence Σ * N) :=
+    or_relation (ltof (sentence Σ) length) (flip (succ G)).
+
+  Lemma sig_lt_wf :
+    wf sig_lt.
+  Proof.
+    intros. apply or_relation_wf.
+    - apply well_founded_ltof.
+    - by apply acyclic_succ_flip_wf.
+  Qed.
+
+  Definition nonempty_partition w : list (sentence Σ * sentence Σ) :=
+    match w with
+    | [] => []
+    | _ :: w' => (λ k, (take k w, drop k w)) <$> (nat_range (length w'))
+    end.
+
+  Lemma nonempty_partition_decrease w wl wr :
+    (wl, wr) ∈ nonempty_partition w →
+    length wl < length w ∧ length wr < length w.
+  Proof.
+    destruct w.
+    - inversion 1.
+    - intros Hin. apply elem_of_list_fmap in Hin as [x [Hp Hx]].
+      inversion Hp; subst; clear Hp.
+      apply nat_range_elem_of in Hx.
+      rewrite take_length drop_length cons_length. lia.
+  Qed.
+
+  Lemma nonempty_partition_spec w wl wr :
+    (wl, wr) ∈ nonempty_partition w ↔
+    w = wl ++ wr ∧ wl ≠ [] ∧ wr ≠ [].
+  Admitted.
+
+  Program Fixpoint check_derive A w {measure (w, A) sig_lt} : bool :=
+    big_or (clauses G A) (λ p, match p with existT α Hα =>
+      match α with
+      | ε => bool_decide (w = [])
+      | atom a =>
+        match w with
+        | [tk] => bool_decide (letter tk = a)
+        | _ => false
+        end
+      | unary B φ => apply₁ φ w && check_derive B w
+      | binary Bl Br φ =>
+        when (G ⊨ Bl ⇒ []) (λ _, check_derive Br w) ||
+        when (G ⊨ Br ⇒ []) (λ _, check_derive Bl w) ||
+        big_or (nonempty_partition w)
+          (λ wp, match wp with existT (wl, wr) Hwp =>
+            apply₂ φ wl wr && check_derive Bl wl && check_derive Br wr
+          end)
+      end
+    end).
+  Next Obligation.
+    intros. naive_solver.
+  Qed.
+  Next Obligation.
+    intros. naive_solver.
+  Qed.
+  Next Obligation.
+    intros. subst. right; split => //.
+    eapply succ_unary; eauto.
+  Qed.
+  Next Obligation.
+    intros. subst. right; split => //.
+    eapply succ_right; eauto.
+  Qed.
+  Next Obligation.
+    intros. subst. right; split => //.
+    eapply succ_left; eauto.
+  Qed.
+  Next Obligation.
+    intros. subst. left.
+    simpl in *.
+    edestruct nonempty_partition_decrease; eauto.
+  Qed.
+  Next Obligation.
+    intros. subst. left.
+    simpl in *.
+    edestruct nonempty_partition_decrease; eauto.
+  Qed.
+  Next Obligation.
+    by apply measure_wf, sig_lt_wf.
+  Qed.
+
+  (* equation lemma *)
+  Lemma check_derive_equation A w :
+    check_derive A w =
+    big_or (clauses G A) (λ p, match p with existT α Hα =>
+      match α with
+      | ε => bool_decide (w = [])
+      | atom a =>
+        match w with
+        | [tk] => bool_decide (letter tk = a)
+        | _ => false
+        end
+      | unary B φ => apply₁ φ w && check_derive B w
+      | binary Bl Br φ =>
+        when (G ⊨ Bl ⇒ []) (λ _, check_derive Br w) ||
+        when (G ⊨ Br ⇒ []) (λ _, check_derive Bl w) ||
+        big_or (nonempty_partition w)
+          (λ wp, match wp with existT (wl, wr) Hwp =>
+            apply₂ φ wl wr && check_derive Bl wl && check_derive Br wr
+          end)
+      end
+    end).
+  Admitted.
+
+  Lemma check_derive_spec A w :
+    check_derive A w = true ↔ G ⊨ A ⇒ w.
+  Proof.
+    split; intros H.
+    - (* -> *)
+      generalize dependent A.
+      induction w as [w IHw] using (well_founded_induction (well_founded_ltof (sentence Σ) length)).
+      induction A as [A IHA] using (well_founded_induction (acyclic_succ_flip_wf _ _ _ acyclic0)).
+      rewrite check_derive_equation big_or_true.
+      intros [[α Hp] Hα]. case_match; subst.
+      + apply bool_decide_eq_true in Hα. subst.
+        by apply derive_ε.
+      + repeat case_match => //.
+        apply bool_decide_eq_true in Hα. subst.
+        destruct t. by apply derive_atom.
+      + apply andb_true_iff in Hα as [? ?].
+        eapply derive_unary; eauto.
+        clear IHw. apply IHA; eauto.
+        eapply succ_unary; eauto.
+      + apply orb_true_iff in Hα as [Hα|Hα].
+        apply orb_true_iff in Hα as [Hα|Hα].
+        * apply when_true in Hα as [Hn ?]. destruct b.
+          rewrite <-app_nil_l. eapply derive_binary; eauto.
+          clear IHw. apply IHA; eauto.
+          eapply succ_right; eauto.
+        * apply when_true in Hα as [Hn ?]. destruct b.
+          rewrite <-app_nil_r. eapply derive_binary; eauto.
+          clear IHw. apply IHA; eauto.
+          eapply succ_left; eauto.
+        * apply big_or_true in Hα as [[[wl wr] Hpar] Hα].
+          apply andb_true_iff in Hα as [Hα ?].
+          apply andb_true_iff in Hα as [? ?].
+          edestruct nonempty_partition_decrease; eauto.
+          edestruct nonempty_partition_spec as [[Hw _] _]; eauto.
+          rewrite Hw. eapply derive_binary; eauto.
+    - (* <- *)
+      destruct H as [t [? [? Ht]]].
+      generalize dependent A.
+      generalize dependent w.
+      induction t; intros.
+      all: inversion Ht; subst; clear Ht.
+      all: rewrite check_derive_equation.
+      all: apply big_or_true.
+      + exists (existT ε H2).
+        apply bool_decide_eq_true. done. 
+      + exists (existT (atom a) H2).
+        repeat case_match => //.
+        apply bool_decide_eq_true. naive_solver.
+      + exists (existT (unary (tree_root t) φ) H3).
+        apply andb_true_iff. naive_solver.
+      + exists (existT (binary (tree_root t1) (tree_root t2) φ) H4).
+        destruct (decide (tree_word t1 = []));
+          last destruct (decide (tree_word t2 = [])).
+        * have Hn : G ⊨ tree_root t1 ⇒ [].
+          { exists t1. by repeat split. }
+          apply orb_true_iff. left.
+          apply orb_true_iff. left.
+          apply when_true. exists Hn.
+          simpl in *. rewrite e app_nil_l. naive_solver.
+        * have Hn : G ⊨ tree_root t2 ⇒ [].
+          { exists t2. by repeat split. }
+          apply orb_true_iff. left.
+          apply orb_true_iff. right.
+          apply when_true. exists Hn.
+          simpl in *. rewrite e app_nil_r. naive_solver.
+        * apply orb_true_iff. right.
+          apply big_or_true. simpl in *.
+          have Hw : (tree_word t1, tree_word t2) ∈ nonempty_partition (tree_word t1 ++ tree_word t2).
+          { apply nonempty_partition_spec. naive_solver. }
+          exists (existT (tree_word t1, tree_word t2) Hw).
+          apply andb_true_iff. split.
+          apply andb_true_iff. split.
+          all: naive_solver.
+  Qed.
+
+  Global Instance acyclic_derive_dec A w :
+    Decision (G ⊨ A ⇒ w).
+  Proof.
+    destruct (check_derive A w) eqn:Heqn.
+    - left. eapply check_derive_spec; eauto.
+    - right. apply not_true_iff_false in Heqn. intros ?.
+      by apply Heqn, check_derive_spec.
+  Qed.
+
+  Program Fixpoint check_reach A w H h {measure (w, A) sig_lt} : bool :=
+    bool_decide (A = H ∧ w = h) ||
+    big_or (clauses G A) (λ p, match p with existT α Hα =>
+      match α with
+      | unary B φ => apply₁ φ w && check_reach B w H h
+      | binary Bl Br φ =>
+        when (G ⊨ Bl ⇒ []) (λ _, check_reach Br w H h) ||
+        (* TODO: h = [] ? *)
+        when (G ⊨ Br ⇒ []) (λ _, check_reach Bl w H h) ||
+        big_or (nonempty_partition w)
+          (λ wp, match wp with existT (wl, wr) Hwp =>
+            apply₂ φ wl wr &&
+            ((check_reach Bl wl H h && bool_decide (G ⊨ Br ⇒ wr))) ||
+            ((bool_decide (G ⊨ Bl ⇒ wl) && check_reach Br wr H h))
+          end)
+      | _ => false
+      end
+    end).
+  Next Obligation.
+    intros. subst. right; split => //.
+    eapply succ_unary; eauto.
+  Qed.
+  Next Obligation.
+    intros. subst. right; split => //.
+    eapply succ_right; eauto.
+  Qed.
+  Next Obligation.
+    intros. subst. right; split => //.
+    eapply succ_left; eauto.
+  Qed.
+  Next Obligation.
+    intros. subst. left.
+    simpl in *.
+    edestruct nonempty_partition_decrease; eauto.
+  Qed.
+  Next Obligation.
+    intros. subst. left.
+    simpl in *.
+    edestruct nonempty_partition_decrease; eauto.
+  Qed.
+  Next Obligation.
+    naive_solver.
+  Qed.
+  Next Obligation.
+    naive_solver.
+  Qed.
+  Next Obligation.
+    by apply measure_wf, sig_lt_wf.
+  Qed.
+
+  Lemma check_reach_equation A w H h :
+    check_reach A w H h =
+    bool_decide (A = H ∧ w = h) ||
+    big_or (clauses G A) (λ p, match p with existT α Hα =>
+      match α with
+      | unary B φ => apply₁ φ w && check_reach B w H h
+      | binary Bl Br φ =>
+        when (G ⊨ Bl ⇒ []) (λ _, check_reach Br w H h) ||
+        when (G ⊨ Br ⇒ []) (λ _, check_reach Bl w H h) ||
+        big_or (nonempty_partition w)
+          (λ wp, match wp with existT (wl, wr) Hwp =>
+            apply₂ φ wl wr &&
+            ((check_reach Bl wl H h && bool_decide (G ⊨ Br ⇒ wr)) ||
+             (bool_decide (G ⊨ Bl ⇒ wl) && check_reach Br wr H h))
+          end)
+      | _ => false
+      end
+    end).
+  Admitted.
+
+  Lemma reachable_sub_sentence A w H h :
+    reachable G A w H h → h `sublist_of` w.
+  Admitted.
+
+  Lemma check_reach_spec A w H h :
+    h ≠ [] →
+    check_reach A w H h = true ↔ reachable G A w H h.
+  Proof.
+    intros Hh.
+    split; intros He.
+    - (* -> *)
+      generalize dependent A.
+      induction w as [w IHw] using (well_founded_induction (well_founded_ltof (sentence Σ) length)).
+      induction A as [A IHA] using (well_founded_induction (acyclic_succ_flip_wf _ _ _ acyclic0)).
+      rewrite check_reach_equation orb_true_iff bool_decide_eq_true big_or_true.
+      intros [[? ?]|Hα]. by constructor.
+      destruct Hα as [[α Hp] Hα]. case_match; subst; try done.
+      + apply andb_true_iff in Hα as [? ?].
+        eapply reachable_unary; eauto.
+        clear IHw. apply IHA; eauto.
+        eapply succ_unary; eauto.
+      + apply orb_true_iff in Hα as [Hα|Hα].
+        apply orb_true_iff in Hα as [Hα|Hα].
+        * apply when_true in Hα as [Hn ?]. destruct b.
+          have -> : w = [] ++ w by rewrite app_nil_l.
+          eapply reachable_right; eauto.
+          clear IHw. apply IHA; eauto.
+          eapply succ_right; eauto.
+        * apply when_true in Hα as [Hn ?]. destruct b.
+          have -> : w = w ++ [] by rewrite app_nil_r.
+          eapply reachable_left; eauto.
+          clear IHw. apply IHA; eauto.
+          eapply succ_left; eauto.
+        * apply big_or_true in Hα as [[[wl wr] Hpar] Hα].
+          apply andb_true_iff in Hα as [? Hα].
+          apply orb_true_iff in Hα as [Hα|Hα].
+          all: apply andb_true_iff in Hα as [? ?].
+          all: edestruct nonempty_partition_decrease; eauto.
+          all: edestruct nonempty_partition_spec as [[Hw _] _]; eauto.
+          all: rewrite Hw.
+          ** eapply reachable_left; eauto. by eapply bool_decide_eq_true.
+          ** eapply reachable_right; eauto. by eapply bool_decide_eq_true.
+    - (* <- *)
+      generalize dependent A.
+      generalize dependent w.
+      induction 1; subst; intros.
+      all: rewrite check_reach_equation orb_true_iff.
+      1: left. 2-4: right; apply big_or_true.
+      + by rewrite bool_decide_eq_true.
+      + exists (existT (unary B φ) H0).
+        apply andb_true_iff. naive_solver.
+      + exists (existT (binary Bl Br φ) H0).
+        have ? : w1 ≠ [].
+        { intros ->.
+          apply reachable_sub_sentence, sublist_nil_r in He.
+          contradiction. }
+        destruct (decide (w2 = [])).
+        * apply orb_true_iff. left.
+          apply orb_true_iff. right.
+          have Hn : G ⊨ Br ⇒ [] by congruence.
+          apply when_true. exists Hn.
+          rewrite e app_nil_r. naive_solver.
+        * apply orb_true_iff. right.
+          apply big_or_true. simpl in *.
+          have Hw : (w1, w2) ∈ nonempty_partition (w1 ++ w2).
+          { apply nonempty_partition_spec. naive_solver. }
+          exists (existT (w1, w2) Hw).
+          apply andb_true_iff. split => //.
+          apply orb_true_iff. left. apply andb_true_iff.
+          split; [naive_solver | by apply bool_decide_eq_true].
+      + exists (existT (binary Bl Br φ) H0).
+        have ? : w2 ≠ [].
+        { intros ->.
+          apply reachable_sub_sentence, sublist_nil_r in He.
+          contradiction. }
+        destruct (decide (w1 = [])).
+        * apply orb_true_iff. left.
+          apply orb_true_iff. left.
+          have Hn : G ⊨ Bl ⇒ [] by congruence.
+          apply when_true. exists Hn.
+          rewrite e app_nil_l. naive_solver.
+        * apply orb_true_iff. right.
+          apply big_or_true. simpl in *.
+          have Hw : (w1, w2) ∈ nonempty_partition (w1 ++ w2).
+          { apply nonempty_partition_spec. naive_solver. }
+          exists (existT (w1, w2) Hw).
+          apply andb_true_iff. split => //.
+          apply orb_true_iff. right. apply andb_true_iff.
+          split; [by apply bool_decide_eq_true | naive_solver].
+  Qed.
+
+End decidability.
