theories/util.v
@@ -1,0 +1,82 @@
+From stdpp Require Import relations.
+From Coq Require Import ssreflect.
+
+Definition or_relation {A B : Type} (R1 : relation A) (R2 : relation B) : relation (A * B) :=
+  λ x y, R1 x.1 y.1 ∨ (x.1 = y.1 ∧ R2 x.2 y.2).
+
+Lemma or_relation_wf {A B : Type} (R1 : relation A) (R2 : relation B) :
+  wf R1 →
+  wf R2 →
+  wf (or_relation R1 R2).
+Proof.
+  intros HR1 HR2 [a b].
+  generalize dependent b.
+  induction a as [a IHa] using (well_founded_induction HR1).
+  induction b as [b IHb] using (well_founded_induction HR2).
+  constructor => [[a' b'] [|]]; naive_solver.
+Qed.
+
+Fixpoint nat_range (n : nat) :=
+  match n with
+  | 0 => []
+  | S n' => nat_range n' ++ [n]
+  end.
+
+Lemma nat_range_length n :
+  length (nat_range n) = n.
+Proof.
+  induction n => //=.
+  rewrite app_length /=. lia.
+Qed.
+
+Lemma nat_range_lookup n i :
+  i < n →
+  nat_range n !! i = Some (S i).
+Proof.
+  intros. induction n; first lia.
+  simpl. destruct (decide (i = n)) as [->|].
+  - rewrite lookup_app_r nat_range_length //.
+    by rewrite Nat.sub_diag.
+  - have ? : i < n by lia.
+    rewrite lookup_app_l ?nat_range_length; naive_solver.
+Qed.
+
+Lemma nat_range_elem_of n x :
+  x ∈ nat_range n → 0 < x ≤ n.
+Proof.
+  intros Hx. apply elem_of_list_lookup in Hx as [i Hi].
+  have ? : i < n.
+  { rewrite <- nat_range_length. eapply lookup_lt_Some; eauto. }
+  rewrite nat_range_lookup in Hi => //.
+  inversion Hi; subst; clear Hi. lia.
+Qed.
+
+Program Fixpoint big_or {A : Type} (l : list A) (P : {x : A & x ∈ l} → bool) : bool :=
+    match l with
+    | [] => false
+    | x :: xs => P (existT x _) || big_or xs (λ y,
+      match y with existT x Hx => P (existT x _) end)
+    end.
+  Next Obligation.
+    intros. subst. apply elem_of_cons. by left.
+  Qed.
+  Next Obligation.
+    intros. subst. apply elem_of_cons. by right.
+  Qed.
+
+Lemma big_or_true {A : Type} (l : list A) (P : {x : A & x ∈ l} → bool) :
+  big_or l P = true ↔ ∃ p, P p = true.
+Admitted.
+
+Program Definition when (P : Prop) `{Decision P} (body : P → bool) : bool :=
+  match bool_decide P with
+  | true => body _
+  | false => false
+  end.
+Next Obligation.
+  intros. eapply bool_decide_eq_true. done.
+Qed.
+
+Lemma when_true P `{Decision P} b :
+  when P b = true ↔ ∃ HP : P, b HP = true.
+Admitted.
